Weidenbach_Book/IsaSAT/IsaSAT_Stats_LLVM.thy
@@ -844,6 +844,87 @@ sepref_def clss_size_incr_lcount_fast_code
   apply (annot_unat_const \<open>TYPE(64)\<close>)
   by sepref
 
+
+sepref_def end_of_restart_phase_impl
+  is \<open>RETURN o end_of_restart_phase_stats\<close>
+  :: \<open>heuristic_int_assn\<^sup>k \<rightarrow>\<^sub>a word_assn\<close>
+  unfolding end_of_restart_phase_stats_def heuristic_int_assn_def
+  by sepref
+
+lemma end_of_restart_phase_stats_end_of_restart_phase:
+  \<open>(end_of_restart_phase_stats, end_of_restart_phase) \<in> heur_rel \<rightarrow> word_rel\<close>
+  by (auto simp: end_of_restart_phase_def code_hider_rel_def)
+
+lemmas end_of_restart_phase_impl_refine[sepref_fr_rules] =
+  end_of_restart_phase_impl.refine[FCOMP end_of_restart_phase_stats_end_of_restart_phase,
+    unfolded heuristic_assn_alt_def[symmetric]]
+
+lemma incr_restart_phase_end_stats_alt_def:
+  \<open>incr_restart_phase_end_stats = (\<lambda>(fast_ema, slow_ema, (ccount, ema_lvl, restart_phase, end_of_phase, length_phase), wasted).
+  (fast_ema, slow_ema, (ccount, ema_lvl, restart_phase, end_of_phase + length_phase, (length_phase * 3) >> 1), wasted))\<close>
+  by auto
+
+sepref_def incr_restart_phase_end_stats_impl [llvm_inline]
+  is \<open>RETURN o incr_restart_phase_end_stats\<close>
+  :: \<open>heuristic_int_assn\<^sup>d \<rightarrow>\<^sub>a heuristic_int_assn\<close>
+  supply[[goals_limit=1]]
+  unfolding heuristic_int_assn_def incr_restart_phase_end_stats_alt_def
+  apply (annot_snat_const \<open>TYPE(64)\<close>)
+  by sepref
+
+sepref_def incr_restart_phase_end_impl
+  is \<open>RETURN o incr_restart_phase_end\<close>
+  :: \<open>heuristic_assn\<^sup>d \<rightarrow>\<^sub>a heuristic_assn\<close>
+  supply[[goals_limit=1]]
+  unfolding incr_restart_phase_end_def
+  by sepref
+
+lemma incr_restart_phase_stats_alt_def:
+  \<open>incr_restart_phase_stats =
+  (\<lambda>(fast_ema, slow_ema, (ccount, ema_lvl, restart_phase, end_of_phase), wasted, \<phi>).
+  (fast_ema, slow_ema, (ccount, ema_lvl, restart_phase XOR 1, end_of_phase), wasted, \<phi>))\<close>
+  by (auto)
+
+sepref_def incr_restart_phase_stats_impl
+  is \<open>RETURN o incr_restart_phase_stats\<close>
+  :: \<open>heuristic_int_assn\<^sup>d \<rightarrow>\<^sub>a heuristic_int_assn\<close>
+  unfolding heuristic_int_assn_def incr_restart_phase_stats_alt_def
+  by sepref
+
+sepref_def incr_restart_phase_impl
+  is \<open>RETURN o incr_restart_phase\<close>
+  :: \<open>heuristic_assn\<^sup>d \<rightarrow>\<^sub>a heuristic_assn\<close>
+  unfolding incr_restart_phase_def
+  by sepref
+
+sepref_def get_restart_count_impl
+  is \<open>RETURN o get_restart_count_stats\<close>
+  :: \<open>stats_int_assn\<^sup>k \<rightarrow>\<^sub>a word_assn\<close>
+  unfolding get_restart_count_stats_def
+  by sepref
+
+lemma get_restart_count_stats_get_restart_count:
+  \<open>(get_restart_count_stats, get_restart_count) \<in> stats_rel \<rightarrow> word_rel\<close>
+  by (auto simp: code_hider_rel_def get_restart_count_def)
+
+lemmas get_restart_count_impl_refine[sepref_fr_rules] =
+  get_restart_count_impl.refine[FCOMP get_restart_count_stats_get_restart_count,
+  unfolded stats_assn_alt_def[symmetric]]
+
+sepref_def get_lrestart_count_impl
+  is \<open>RETURN o get_lrestart_count_stats\<close>
+  :: \<open>stats_int_assn\<^sup>k \<rightarrow>\<^sub>a word_assn\<close>
+  unfolding get_lrestart_count_stats_def
+  by sepref
+
+lemma get_lrestart_count_stats_get_lrestart_count:
+  \<open>(get_lrestart_count_stats, get_lrestart_count) \<in> stats_rel \<rightarrow> word_rel\<close>
+  by (auto simp: code_hider_rel_def get_lrestart_count_def)
+
+lemmas get_lrestart_count_impl_refine[sepref_fr_rules] =
+  get_lrestart_count_impl.refine[FCOMP get_lrestart_count_stats_get_lrestart_count,
+  unfolded stats_assn_alt_def[symmetric]]
+
 sepref_register unset_fully_propagated_heur is_fully_propagated_heur set_fully_propagated_heur
 
 end
